# Lebesgue integrals and Riemann-Stieltjes integral

#### recall: Riemann Stieljes integral
Assume that $\omega(x)$ is a bounded variation function on $[a,b]$, it is known that $\omega = \omega^++\omega^-$, where $\omega^+,\omega^-$ are nondecreasing functions.

Let $f(x)$ be bounded inn $[a,b]$, then the Riemann-Stieltjes integral $\int_a^b f(x)d\omega^+$ or $\int_a^b f(x)d\omega^-$ are defined in the Riemann sense.
That is, Let $P=\{a=x_0<x_1<...<x_n=b\}$ be a partition of $[a,b]$, the Riemann sum $R^\pm(P)=\sum_{k=1}^n f(x_k^*) [\omega^\pm (x_k)-\omega^\pm(x_{k-1})]$

$\int_a^b f(x)d\omega^\pm = \lim_{|P|\to 0}R^\pm(P)$

$\implies \int_a^b f(x)d\omega = \int_a^b f(x)d\omega^+ - \int_a^b f(x)d\omega^-$

## Theorem
if $f(x)$ is continuous on $[a,b]$ and $\omega$ is of b.v. on $[a,b]$
then $\int_a^b f(x)d\omega(x)$ exist

Let $f$ be the Lebesgue measurable function on $E\subseteq \mathbb R^n$ ($E$ is measurable)

## Def.
Let $-\infty <a < \infty$, define the distribution function of $f$ on $E$ is given by 
$\omega_{f, E}(a)=\omega(a)=\{x\in E:f(x)>a\}$

### properties
1. $\omega(a)$ is non-increasing
2. $\lim_{a\to \infty} \omega(a)=0$ unless $\omega(a)=\infty \forall a$
To avoid this, we assume that $|E|<\infty$ and $f$ is finite a.e. (if $|\{f=\infty\}|>0$, then $\lim_{a\to\infty} \omega(a)\neq 0$)

3. $\lim_{a\to-\infty} \omega(a)=|E|$ ( $f>-\infty$ a.e. )

4. $\omega(a)$ is of bounded variation.


### Lemma.1
if $\alpha<\beta$, then $|\{\alpha < f\le \beta\}|=\omega(\alpha)-\omega(\beta)$


### Lemma.2

Given $\alpha\in\mathbb R$, define $\omega(\alpha+)= \lim_{\epsilon\to 0^+} \omega(\alpha+\epsilon), \omega(\alpha-)=\lim_{\epsilon\to 0^+}omega(\alpha - \epsilon)$

1. $\omega(\alpha+)=\omega(\alpha)$ i.w. $\omega(\alpha)$ is continuous from the right.
2. $\omega(\alpha-)=|\{f\ge \alpha\}|$

proof.
1. $\omega(\alpha+)=\lim_{\epsilon\to 0^+} \omega(\alpha+\epsilon)= \lim_{\epsilon\to 0^+} |\{f>\alpha+\epsilon\}|$
Note that $\{f>\alpha+\epsilon\}\to \{f>\alpha\}$ by continuity of measure
$\implies \omega(\alpha+\epsilon)\to \omega(\alpha)$

2. trivial

#### remark
1. $\omega(\alpha)$ is non-increasing function which is continuous from the right and may have jump discontinuities with jumps $\omega(\alpha-) - \omega(\alpha+)>0$

2. $\omega$ is continuous if and only if $|\{f=\alpha\}|=0$

3. $\omega$ is constant in an open interval $(\alpha,\beta)$ if and only if $|\{\alpha<f<\beta\}|=0$
that is, iff $f$ takes almost no values between $\alpha$ and $\beta$

## Theorem
If $a<f(x)<b$, ( $a,b$ finite ), then
$\underbrace {\int_E fdx}_{\rm Lebesgue}=\underbrace{-\int_a^b \alpha d\omega(\alpha)}_{\rm Riemann-Stieltjes}$

proof.
Let $P=\{a = \alpha_0<\alpha_1<...<\alpha_n = b\}$ be any partition of $[a,b]$,
Let $E_j=\{\alpha_{j-1} < f(x)\le \alpha_j\}$

then $|E_j|= |\{\alpha_{j-1} < f(x)\le \alpha_j\}|=\omega(\alpha_{j-1})-\omega(\alpha_j)$

$E=\cup_{j=1}^n E_j$, and $E_j$ disjoint.
Hence, $\sum_{j=1}^n \alpha_{j-1} |E_j|\le \int_E f(x) \le \sum_{j=1}^n \alpha_j |E_j|$

$\implies -\sum_{j=1}^n \alpha_{j-1}[\omega(\alpha_j)-\omega(\alpha_{j-1})] \le \int_E fdx \le -\sum_{j=1}^n \alpha_{j}[\omega(\alpha_j)-\omega(\alpha_{j-1})]$

take $n\to\infty\implies \int_E fdx = -\int_a^b \alpha d\omega(\alpha)$

### Corollary
Let $f$ be measurable on $E$, define $E_{ab}=\{x\in E:a< f(x)\le b\}$, a,b finite.
Then $\int_{E_{ab}} fdx=-\int_a^b \alpha d\omega(\alpha)$

proof.
$\omega_{f, E}(\alpha) = |\{x\in E:f(x)>\alpha\}|$

$\omega_{f, E_{ab}}(\alpha)=|x\in E_{ab}:f(x)>\alpha|$
But $\omega_{f, E_{ab}}(\alpha)-\omega_{f, E_{ab}}(\beta)=\omega_{f, E}(\alpha)-\omega_{f, E}(\beta)$
Therefore, the Corollary follows.

Let $f$ be measurable on $E$, $|E|<\infty$

Define $-\int_{-\infty}^\infty \alpha d\omega(\alpha)=\lim_{a\to -\infty, b\to\infty} \left(-\int_a^b \alpha d\omega(\alpha)\right)$

provided the limit exist.

proof.
#### 1. 
Assume that $\int_E f$ is finite u.e. $f\in L(E)$
in other wordsm $\int_E f^+$ and $\int_E f^-$ finite.

Recall that $\int_E \chi_{E_{ab}} fdx=\int_{E_{ab}} fdx= -\int_a^b  \alpha d\omega(\alpha)$


By the monotone convergence theorem, 
- $f^+ E_{ab}\to f^+$ increasingly
- $f^- E_{ab}\to f^-$ increasingly

Hence, $\int_{E_{ab}} f=\int_{E_{ab}} f^+-\int_{E_{ab}}f^- \to \int_E f^+-\int_E f^- = \int_E f$

so, $\int_{E_{ab}} f\stackrel{a\to-\infty, b\to\infty}{\to} \int_E f$

#### 2. 
Assume that $\int_{-\infty}^\infty \alpha d\omega(\alpha)$ is finite, so $\int_0^\infty \alpha d\omega(\alpha)$ and $\int_{-\infty}^0 \alpha d\omega(\alpha)$ are finite.

###### claim
$\int_E f^+=-\int_0^\infty \alpha d\omega(\alpha)$ and $\int_E f^-=-\int_{-\infty}^0 \alpha d\omega(\alpha)$

proof.
for $b>0$, $\int_{E_{0b}} f = -\int_0^b \alpha d\omega(\alpha)\stackrel{b\to\infty}{\to }-\int_0^\infty \alpha d\omega(\alpha)$

By the monotone convergence, $\int_{E_{0b}} f=\int_{E_{0b}} f^+ \to \int_{\{0<f<\infty\}} f^+$ increasingly.

So, $\int_{\{ 0<f<\infty\}} f^+ =-\int_0^\infty \alpha d\omega(\alpha)$

similarly, $\int_{\{-\infty < f(x)\le 0\}} f^- = -\int_{-\infty}^0 \alpha d\omega(\alpha)$

# Composite function
## Theorem
Let $a<f\le b$ $\forall x\in E$, Assume that $\phi$ is continuous on $[a,b]$, then
$\int_E \phi(f)=-\int_a^b  \phi(\alpha) d \omega(\alpha)$

proof: EXERCISE

## Theorem
Let $\phi$ be continuous on $(-\infty, \infty)$, if $\phi(f) \in L(E)$, then
$\int_{-\infty}^\infty \phi(\alpha)d\omega(\alpha)$ is finite ($\int_{-\infty}^\infty \phi(\alpha)d\omega(\alpha)=\int_{a\to -\infty, b\to\infty} \phi(f)d\omega(\alpha)$)

and $\int_E \phi(f)=-\int_{-\infty}^\infty \phi(\alpha)d\omega(\alpha)$

proof:EXERCISE

